fixing and adding back wysteria

lib/ordset.fsi
@@ -1,4 +1,4 @@
-(*--build-config
+(*--Build-config
 
  --*)
 module FStar.OrdSet
@@ -83,9 +83,9 @@ val eq_remove: #a:Type -> #f:cmp a -> x:a -> s:ordset a f
                         (ensures (s = remove #a #f x s))
                   [SMTPat (remove #a #f x s)]
 
-val size_empty: #a:Type -> #f:cmp a
-                -> Lemma (requires True) (ensures (size #a #f (empty #a #f) = 0))
-                   [SMTPat (size #a #f (empty #a #f))]
+val size_empty: #a:Type -> #f:cmp a -> s:ordset a f
+                -> Lemma (requires True) (ensures ((size #a #f s = 0) = (s = empty #a #f)))
+                  [SMTPat (size #a #f s)]
                    
 val size_remove: #a:Type -> #f:cmp a -> y:a -> s:ordset a f
                  -> Lemma (requires (mem #a #f y s))
@@ -96,10 +96,6 @@ val size_singleton: #a:Type -> #f:cmp a -> x:a
                     -> Lemma (requires True) (ensures (size #a #f (singleton #a #f x) = 1))
                        [SMTPat (size #a #f (singleton #a #f x))]
                        
-val s_eq_empty: #a:Type -> #f:cmp a -> s:ordset a f
-                -> Lemma (requires True) (ensures ((size #a #f s = 0) = (s = empty)))
-                   [SMTPat (s = empty)]
-
 (* TODO:FIXME: implement *)
 val size_union: #a:Type -> #f:cmp a -> s1:ordset a f -> s2:ordset a f
                 -> Lemma (requires True)
